wip

cedar-lean/Cedar/Thm/EntitySlice.lean
@@ -455,7 +455,88 @@ theorem well_typed_without_euids_list (ty : CedarType) (list : List Value)
     repeat assumption
 
 
-theorem well_typed-without_euids_record (map_values : List (Attr × ))
+
+
+
+theorem well_typed_without_euids_record' (map_values : List (Attr × Value)) (map_types : List (Attr × QualifiedType))
+  (well_typed : ∀ k v, (k,v) ∈  map_values → ∃ ty, (k, ty) ∈ map_types ∧ InstanceOfType v ty.getType ∧ NoEuidTypesIn ty.getType )
+  (ih : ∀ ty k v, (k,v) ∈ map_values → InstanceOfType v ty → NoEuidTypesIn ty → NoEuidValues v)
+  :
+  NoEuidValuesInRecord map_values
+  := by
+  induction map_values
+  case nil =>
+    constructor
+  case cons head tail local_ih =>
+    have ⟨key, value⟩ := head
+    have ⟨ty, in_record_type, instance_of, no_euids⟩  := well_typed key value (by simp)
+    constructor
+    case _ =>
+      apply ih
+      simp
+      apply Or.inl
+      rfl
+      apply instance_of
+      apply no_euids
+    case _ =>
+      apply local_ih
+      intros k v in_tail
+      have ⟨ty, step⟩ : ∃ ty, (k, ty) ∈ map_types ∧ InstanceOfType v ty.getType ∧ NoEuidTypesIn ty.getType := by
+        apply well_typed
+        simp [in_tail]
+      exists ty
+      intros ty k v in_tail instance_of no_euids
+      apply ih
+      simp
+      apply Or.inr
+      apply in_tail
+      apply instance_of
+      apply no_euids
+
+
+
+
+theorem well_typed_without_euids_record (map_values : List (Attr × Value)) (map_types : List (Attr × QualifiedType))
+  (well_typed : InstanceOfType  (.record (.mk map_values)) (.record (.mk map_types)))
+  (no_euids_in_type : NoEuidTypesInList map_types)
+  (ih : ∀ ty k v, (k,v) ∈ map_values → InstanceOfType v ty → NoEuidTypesIn ty → NoEuidValues v)
+  :
+  NoEuidValuesInRecord map_values
+  := by
+  cases well_typed
+  rename_i h₁ h₂ h₃
+  apply well_typed_without_euids_record'
+  intros k v in_values
+  have ⟨ty, in_type⟩ : ∃ ty, (k,ty) ∈ map_types := by
+    have step : (Map.mk map_types).contains k = true := by
+      apply h₁
+      rw [Map.contains_iff_some_find?]
+      apply Map.in_mk_in_map
+      apply in_values
+    apply Map.in_list_if_contains
+    apply step
+  exists ty
+  constructor
+  case _ =>
+    apply in_type
+  case _ =>
+    constructor
+    case _ =>
+      apply h₂
+      apply (Map.in_list_iff_find?_some ?_).mp
+      simp [Map.kvs]
+
+      sorry
+    case _ =>
+      sorry
+
+
+
+
+
+
+  sorry
+
 
 
 theorem well_typed_without_euids (ty : CedarType) (v : Value)
@@ -490,6 +571,7 @@ theorem well_typed_without_euids (ty : CedarType) (v : Value)
     apply well_typed_without_euids
     repeat assumption
   case record map_values =>
+
     cases map_values
     rename_i map_values
     constructor
@@ -497,13 +579,262 @@ theorem well_typed_without_euids (ty : CedarType) (v : Value)
     rename_i rty h₁ h₂ h₃
     cases no_euids
     rename_i map_types h₄
+    apply well_typed_without_euids_record
+    repeat assumption
+    apply InstanceOfType.instance_of_record
+    repeat assumption
+  case _ =>
+    constructor
+termination_by sizeOf v
+decreasing_by
+  case _ =>
+    simp_wf
+    rename Value => v'
+    rename List Value => members
+    rename_i set eq_value _ set' _ _ _ _ _ _ _ _ _ _ _ _ _ _ _ _ _ _
+    rename set = set' => eq
+    subst eq
+    subst eq_value
+    rename set = Set.mk members => set_eq
+    subst set_eq
+    simp
+    have step : sizeOf v' < sizeOf members := by
+      apply List.sizeOf_lt_of_mem
+      assumption
+    omega
+
+theorem no_euids_in_reqty_means_no_euids_in_context : ∀ env request entities l,
+  NoEuidsInEnv env →
+  RequestAndEntitiesMatchEnvironmentLeveled env request entities l →
+  NoEuidsInContext request
+  := by
+  intros env request entities l no_euids well_typed
+  simp [NoEuidsInEnv] at no_euids
+  simp [NoEuidsInContext]
+  apply well_typed_without_euids
+  case _ =>
+    simp [RequestAndEntitiesMatchEnvironmentLeveled, InstanceOfRequestTypeLevel] at well_typed
+    have h₁ := well_typed.left.right.right.right.right.right.right
+    apply h₁
+  case _ =>
+    apply no_euids
 
 
 
+
+def evalsToEuid (e : Expr) : Prop :=
+  ∀ entities request env (c₁ c₂ : Capabilities) ety l euid,
+    typeOf e c₁ env (.finite 1 == Level.infinite) = .ok (.entity ety l, c₂) →
+    l ≠ Level.zero →
+    CapabilitiesInvariant c₁ request entities →
+    RequestAndEntitiesMatchEnvironmentLeveled env request entities (.finite 1) →
+    NoEuidsInEnv env →
+    evaluate e request entities = .ok (Value.prim (.entityUID euid)) →
+    (euid ∈ [request.principal, request.action, request.resource])
+
+theorem evals_to_euid_lit (p : Prim) entities request env c₁ c₂ ety l euid
+  (well_typed : typeOf (.lit p) c₁ env (.finite 1 == Level.infinite) = .ok (.entity ety l, c₂))
+  (non_zero : l ≠ Level.zero)
+  (is_euid : evaluate (.lit p) request entities = .ok (Value.prim (.entityUID euid))) :
+  (euid ∈ [request.principal, request.action, request.resource])
+  := by
+  cases p <;> simp [evaluate] at is_euid
+  case _ =>
+    exfalso
+    simp [typeOf, typeOfLit] at well_typed
+    split at well_typed
+    case _ =>
+      simp [ok] at well_typed
+      replace ⟨well_typed, _⟩ := well_typed
+      replace ⟨_, well_typed⟩ := well_typed
+      rw [if_neg] at well_typed
+      subst well_typed
+      simp [Level.zero] at non_zero
+      unfold Not
+      intros contra
+      cases contra
+    case _ =>
+      simp [err] at well_typed
+
+theorem evals_to_euid_var (v : Var) entities request env c₁ c₂ ety l euid
+  (well_typed : typeOf (.var v) c₁ env (.finite 1 == Level.infinite) = .ok (.entity ety l, c₂))
+  (is_euid : evaluate (.var v) request entities = .ok (Value.prim (.entityUID euid))) :
+  (euid ∈ [request.principal, request.action, request.resource])
+  := by
+  cases v
+    <;>
+    simp [evaluate] at is_euid
+    <;> (
+    subst is_euid
+    simp
+    )
+
+theorem levels_nonzero {l l' : Level}
+  (l_not_zero : l ≠ .finite 0)
+  (l'_ge : l ≤ l') :
+  l' ≠ .finite 0
+  := by
+  cases l <;> cases l' <;> try simp [Level.finite]
+  case _ =>
+    cases l'_ge
+  case _ n₁ n₂ =>
+    have n₁_not_zero : n₁ ≠ 0 := by
+      simp [Level.finite] at l_not_zero
+      omega
+    have step : n₁ ≤ n₂ := by
+      exact Level.le_inversion l'_ge
+    simp [Level.finite]
+    omega
+
+
+
+theorem evals_to_euid_ite (cond cons alt : Expr) entities request env c₁ c₂ ety l euid
+  (well_typed : typeOf (.ite cond cons alt)  c₁ env (.finite 1 == Level.infinite) = .ok (.entity ety l, c₂))
+  (non_zero : l ≠ Level.zero)
+  (caps_inv : CapabilitiesInvariant c₁ request entities)
+  (req_well_typed : RequestAndEntitiesMatchEnvironmentLeveled env request entities (.finite 1))
+  (no_euids : NoEuidsInEnv env)
+  (is_euid : evaluate (.ite cond cons alt) request entities = .ok (Value.prim (.entityUID euid)))
+  (ih₁ : evalsToEuid cons)
+  (ih₂ : evalsToEuid alt) :
+  (euid ∈ [request.principal, request.action, request.resource])
+  := by
+  have ⟨bty, c₁', ty₂, c₂', ty₃, c₃, hinv₁, hinv⟩ := type_of_ite_inversion well_typed
+  have ⟨gcaps_inv, v_cond, sound₁, sound₂⟩ : GuardedCapabilitiesInvariant cond c₁' request entities ∧ ∃ v, EvaluatesToLeveled cond request entities v  ∧ InstanceOfType v (.bool bty) := by
+    apply type_of_is_sound_noninfinite
+    apply LevelLT.finite₂
+    apply 1
+    repeat assumption
+  cases bty
+  case tt =>
+    simp at hinv
+    cases sound₂
+    rename_i bool sound₂
+    simp [InstanceOfBoolType] at sound₂
+    cases bool
+      <;> simp at sound₂
+    rcases sound₁ with evals | evals | evals
+      <;> simp [evals, evaluate, Result.as]  at is_euid
+    case _ =>
+      simp [Coe.coe, Value.asBool] at is_euid
+      have ⟨hinv₂, hinv₃, _⟩ := hinv
+      subst hinv₃
+      apply ih₁
+      repeat assumption
+      apply capability_union_invariant
+      assumption
+      apply gcaps_inv
+      repeat assumption
+  case ff =>
+    simp at hinv
+    cases sound₂
+    rename_i bool sound₂
+    simp [InstanceOfBoolType] at sound₂
+    cases bool
+      <;> simp at sound₂
+    rcases sound₁ with evals | evals | evals
+      <;> simp [evals, evaluate, Result.as, Coe.coe, Value.asBool] at is_euid
+    have ⟨hinv₂, hinv₃, _⟩  := hinv
+    subst hinv₃
+    apply ih₂
+    apply hinv₂
+    apply non_zero
+    repeat assumption
+  case anyBool =>
+    simp at hinv
+    cases sound₂
+    rename_i bool sound₂
+    cases bool
+    case true =>
+      rcases sound₁ with evals | evals | evals
+      <;> simp [evals, evaluate, Result.as, Coe.coe, Value.asBool] at is_euid
+      have ⟨l', step₁⟩ : ∃ l', ty₂ = .entity ety l' := by
+        apply lubs_to_entity ty₃ ty₂ ety l
+        rw [lub_comm]
+        simp [hinv]
+      have typed_as_entity := hinv.left
+      rw [step₁] at typed_as_entity
+      apply ih₁
+      apply typed_as_entity
+      have step₂ : l ≤ l' := by
+        apply lub_to_entity_level_bound ty₃ ety l' l
+        rw [lub_comm]
+        rw [← step₁]
+        simp [hinv]
+      apply levels_nonzero
+      apply non_zero
+      apply step₂
+      apply capability_union_invariant
+      assumption
+      apply gcaps_inv
+      repeat assumption
+    case false =>
+      rcases sound₁ with evals | evals | evals
+      <;> simp [evals, evaluate, Result.as, Coe.coe, Value.asBool] at is_euid
+      have ⟨l', step₁⟩ : ∃ l', ty₃ = .entity ety l' := by
+        apply lubs_to_entity ty₂ ty₃ ety l
+        simp [hinv]
+      have typed_as_entity := hinv.right.left
+      rw [step₁] at typed_as_entity
+      apply ih₂
+      apply typed_as_entity
+      have step₂ : l ≤ l' := by
+        apply lub_to_entity_level_bound ty₂ ety l' l
+        rw [← step₁]
+        simp [hinv]
+      apply levels_nonzero
+      apply non_zero
+      repeat assumption
+
+
+
+
+theorem evals_to_euid (e : Expr) entities request env c₁ c₂ ety l euid
+  (well_typed : typeOf e c₁ env (.finite 1 == Level.infinite) = .ok (.entity ety l, c₂))
+  (non_zero : l ≠ Level.zero)
+  (caps_inv : CapabilitiesInvariant c₁ request entities)
+  (req_well_typed : RequestAndEntitiesMatchEnvironmentLeveled env request entities (.finite 1))
+  (no_euids : NoEuidsInEnv env)
+  (is_euid : evaluate e request entities = .ok (Value.prim (.entityUID euid))) :
+  (euid ∈ [request.principal, request.action, request.resource])
+  := by
+  cases e
+  case lit p =>
+    apply evals_to_euid_lit
+    repeat assumption
+  case var v =>
+    apply evals_to_euid_var
+    repeat assumption
+  case ite cond cons alt =>
+    apply evals_to_euid_ite
+    repeat assumption
+    all_goals {
+      unfold evalsToEuid
+      intros
+      apply evals_to_euid
+      repeat assumption
+    }
+  case and lhs rhs =>
 
     sorry
   case _ =>
     sorry
+  case _ =>
+    sorry
+  case _ =>
+    sorry
+  case _ =>
+    sorry
+  case _ =>
+    sorry
+  case _ =>
+    sorry
+  case _ =>
+    sorry
+  case _ =>
+    sorry
+
+
 
 
 def simpleSlice_soundness (e : Expr) : Prop  :=
@@ -669,6 +1000,7 @@ theorem simpleSlice_is_sound (e : Expr) (entities slice : Entities) (request : R
   (well_typed : typeOf e c₁ env false = .ok (ty, c₂))
   (slice_eq : simpleSlice request entities = .some slice)
   (caps_inv : CapabilitiesInvariant c₁ request entities)
+  (h : noEuidsInEnv env)
   (full_store_typed : RequestAndEntitiesMatchEnvironmentLeveled env request entities (.finite 1)) :
   evaluate e request slice = evaluate e request entities
   := by
@@ -680,21 +1012,12 @@ theorem simpleSlice_is_sound (e : Expr) (entities slice : Entities) (request : R
   case ite cond cons alt =>
     apply simpleSlice_is_sound_ite
     repeat assumption
-    case _ =>
+    all_goals {
       simp [simpleSlice_soundness]
       intros
       apply simpleSlice_is_sound
       repeat assumption
-    case _ =>
-      simp [simpleSlice_soundness]
-      intros
-      apply simpleSlice_is_sound
-      repeat assumption
-    case _ =>
-      simp [simpleSlice_soundness]
-      intros
-      apply simpleSlice_is_sound
-      repeat assumption
+    }
   case and lhs rhs =>
     sorry
   case or lhs rhs =>
